cleaning up

bidirectional/theories/BDTyping.v
@@ -5,8 +5,8 @@ From Coq Require String.
 From MetaCoq.Template Require Import config utils monad_utils.
 From MetaCoq.PCUIC Require Import PCUICAst PCUICAstUtils
   PCUICLiftSubst PCUICUnivSubst PCUICEquality PCUICUtils
-  PCUICCases PCUICPosition PCUICTyping.
-(* From MetaCoq.Bidirectional Require Import BDEnvironmentTyping. *)
+  PCUICPosition PCUICTyping.
+From MetaCoq.Bidirectional Require Import BDEnvironmentTyping.
 
 From MetaCoq Require Export LibHypsNaming.
 Require Import ssreflect.
@@ -23,109 +23,83 @@ Include BDLookup.
 Module BDEnvTyping := EnvTyping PCUICTerm PCUICEnvironment.
 Include BDEnvTyping. *)
 
+
 Notation "Σ ;;; Γ |- t --> t'" := (red Σ Γ t t') (at level 50, Γ, t, t' at next level) : type_scope.
 Reserved Notation " Σ ;;; Γ |- t ▹ T " (at level 50, Γ, t, T at next level).
-Reserved Notation " Σ ;;; Γ |- t ▹□ u " (at level 50, Γ, t, u at next level).
-Reserved Notation " Σ ;;; Γ |- t ▹Π ( na , A , B ) " (at level 50, Γ, t, na, A, B at next level).
-Reserved Notation " Σ ;;; Γ |- t ▹{ ind } ( u , args )" (at level 50, Γ, t, ind, u, args at next level).
+Reserved Notation " Σ ;;; Γ |- t ▸□ u " (at level 50, Γ, t, u at next level).
+Reserved Notation " Σ ;;; Γ |- t ▸Π ( na , A , B ) " (at level 50, Γ, t, na, A, B at next level).
+Reserved Notation " Σ ;;; Γ |- t ▸{ ind } ( u , args )" (at level 50, Γ, t, ind, u, args at next level).
 Reserved Notation " Σ ;;; Γ |- t ◃ T " (at level 50, Γ, t, T at next level).
 
 
 Inductive infering `{checker_flags} (Σ : global_env_ext) (Γ : context) : term -> term -> Type :=
 | infer_Rel n decl :
-    All_local_env (lift_sorting checking infering_sort Σ) Γ ->
     nth_error Γ n = Some decl ->
     Σ ;;; Γ |- tRel n ▹ lift0 (S n) decl.(decl_type)
 
 | infer_Sort s :
-    All_local_env (lift_sorting checking infering_sort Σ) Γ ->
     wf_universe Σ s->
     Σ ;;; Γ |- tSort s ▹ tSort (Universe.super s)
 
 | infer_Prod na A B s1 s2 :
-    Σ ;;; Γ |- A ▹□ s1 ->
-    Σ ;;; Γ ,, vass na A |- B ▹□ s2 ->
+    Σ ;;; Γ |- A ▸□ s1 ->
+    Σ ;;; Γ ,, vass na A |- B ▸□ s2 ->
     Σ ;;; Γ |- tProd na A B ▹ tSort (Universe.sort_of_product s1 s2)
 
 | infer_Lambda na A t s B :
-    Σ ;;; Γ |- A ▹□ s ->
+    Σ ;;; Γ |- A ▸□ s ->
     Σ ;;; Γ ,, vass na A |- t ▹ B ->
     Σ ;;; Γ |- tLambda na A t ▹ tProd na A B
 
 | infer_LetIn na b B t s A :
-    Σ ;;; Γ |- B ▹□ s ->
+    Σ ;;; Γ |- B ▸□ s ->
     Σ ;;; Γ |- b ◃ B ->
     Σ ;;; Γ ,, vdef na b B |- t ▹ A ->
     Σ ;;; Γ |- tLetIn na b B t ▹ tLetIn na b B A
 
 | infer_App t na A B u :
-    Σ ;;; Γ |- t ▹Π (na,A,B) ->
+    Σ ;;; Γ |- t ▸Π (na,A,B) ->
     Σ ;;; Γ |- u ◃ A ->
     Σ ;;; Γ |- tApp t u ▹ B{0 := u}
 
 | infer_Const cst u :
-    All_local_env (lift_sorting checking infering_sort Σ) Γ ->
     forall decl (isdecl : declared_constant Σ.1 cst decl),
     consistent_instance_ext Σ decl.(cst_universes) u ->
     Σ ;;; Γ |- tConst cst u ▹ subst_instance_constr u decl.(cst_type)
 
 | infer_Ind ind u :
-    All_local_env (lift_sorting checking infering_sort Σ) Γ ->
-    forall mdecl idecl (isdecl : declared_inductive Σ.1 ind mdecl idecl),
+    forall mdecl idecl (isdecl : declared_inductive Σ.1 mdecl ind idecl),
     consistent_instance_ext Σ mdecl.(ind_universes) u ->
     Σ ;;; Γ |- tInd ind u ▹ subst_instance_constr u idecl.(ind_type)
 
 | infer_Construct ind i u :
-    All_local_env (lift_sorting checking infering_sort Σ) Γ ->
-    forall mdecl idecl cdecl (isdecl : declared_constructor Σ.1 (ind, i) mdecl idecl cdecl),
+    forall mdecl idecl cdecl (isdecl : declared_constructor Σ.1 mdecl idecl (ind, i) cdecl),
     consistent_instance_ext Σ mdecl.(ind_universes) u ->
     Σ ;;; Γ |- tConstruct ind i u ▹ type_of_constructor mdecl cdecl (ind, i) u
 
-(* | infer_Case (indnpar : inductive × nat) (u : Instance.t) (p c : term) (brs : list (nat × term)) (args : list term) :
+| infer_Case (indnpar : inductive × nat) (u : Instance.t) (p c : term) (brs : list (nat × term)) (args : list term) :
   let ind := indnpar.1 in
   let npar := indnpar.2 in
-   Σ ;;; Γ |- c ▹{ind} (u,args) ->
   forall mdecl idecl (isdecl : declared_inductive Σ.1 mdecl ind idecl),
   mdecl.(ind_npars) = npar ->
   isCoFinite mdecl.(ind_finite) = false ->
+   Σ ;;; Γ |- c ▸{ind} (u,args) ->
   let params := List.firstn npar args in
   forall ps pty, build_case_predicate_type ind mdecl idecl params u ps = Some pty ->
+  wf_universe Σ ps ->
   Σ ;;; Γ |- p ◃ pty ->
-  leb_sort_family (universe_family ps) idecl.(ind_kelim) ->
+  is_allowed_elimination Σ ps (ind_kelim idecl) ->
   forall (btys : list (nat × term)),
   map_option_out (build_branches_type ind mdecl idecl params u p) = Some btys ->
   All2 (fun br bty =>
     (br.1 = bty.1) ×
-    (Σ ;;; Γ |- bty.2 ▹□ ps) ×
     (Σ ;;; Γ |- br.2 ◃ bty.2))
     brs btys ->
-  Σ ;;; Γ |- tCase indnpar p c brs ▹ mkApps p (skipn npar args ++ [c]) *)
-
-| type_Case (ci : case_info) p c brs indices ps :
-  forall mdecl idecl (isdecl : declared_inductive Σ.1 ci.(ci_ind) mdecl idecl),
-  mdecl.(ind_npars) = ci.(ci_npar) ->
-  let predctx := case_predicate_context ci.(ci_ind) mdecl idecl p in
-  wf_predicate mdecl idecl p ->
-  wf_local Σ (Γ ,,, p.(pcontext)) ->
-  conv_context Σ (Γ ,,, p.(pcontext)) (Γ ,,, predctx) ->
-  Σ ;;; Γ ,,, predctx |- p.(preturn) ▹□ ps ->
-  is_allowed_elimination Σ ps idecl.(ind_kelim) ->
-  Σ ;;; Γ |- c ◃ mkApps (tInd ci.(ci_ind) p.(puinst)) (p.(pparams) ++ indices) ->
-  isCoFinite mdecl.(ind_finite) = false ->
-  let ptm := it_mkLambda_or_LetIn predctx p.(preturn) in
-  wf_branches idecl brs ->
-  All2i (fun i cdecl br =>
-    let brctxty := case_branch_type ci.(ci_ind) mdecl idecl p br ptm i cdecl in
-    (wf_local Σ (Γ ,,, br.(bcontext)) ×
-      conv_context Σ (Γ ,,, br.(bcontext)) (Γ ,,, brctxty.1)) ×
-    (Σ ;;; Γ ,,, brctxty.1 |- brctxty.2 ◃ tSort ps) ×
-    (Σ ;;; Γ ,,, brctxty.1 |- br.(bbody) ◃ brctxty.2))
-    0 idecl.(ind_ctors) brs ->
-  Σ ;;; Γ |- tCase ci p c brs ▹ mkApps ptm (indices ++ [c])
+  Σ ;;; Γ |- tCase indnpar p c brs ▹ mkApps p (skipn npar args ++ [c])
 
 | infer_Proj p c u :
-    forall mdecl idecl pdecl (isdecl : declared_projection Σ.1 p mdecl idecl pdecl) (args : list term),
-    Σ ;;; Γ |- c ▹{fst (fst p)} (u,args) ->
+    forall mdecl idecl pdecl (isdecl : declared_projection Σ.1 mdecl idecl p pdecl) (args : list term),
+    Σ ;;; Γ |- c ▸{fst (fst p)} (u,args) ->
     #|args| = ind_npars mdecl ->
     let ty := snd pdecl in
     Σ ;;; Γ |- tProj p c ▹ subst0 (c :: List.rev args) (subst_instance_constr u ty)
@@ -133,18 +107,15 @@ Inductive infering `{checker_flags} (Σ : global_env_ext) (Γ : context) : term 
 | infer_Fix (mfix : mfixpoint term) n decl :
     fix_guard Σ Γ mfix ->
     nth_error mfix n = Some decl ->
-    All_local_env (lift_sorting checking infering_sort Σ) Γ ->
-    All (fun d => {s & Σ ;;; Γ |- d.(dtype) ▹□ s}) mfix ->
-    All (fun d => (Σ ;;; Γ ,,, fix_context mfix |- d.(dbody) ◃ lift0 #|fix_context mfix| d.(dtype))
-      × (isLambda d.(dbody) = true)) mfix ->
+    All (fun d => {s & Σ ;;; Γ |- d.(dtype) ▸□ s}) mfix ->
+    All (fun d => Σ ;;; Γ ,,, fix_context mfix |- d.(dbody) ◃ lift0 #|fix_context mfix| d.(dtype)) mfix ->
     wf_fixpoint Σ.1 mfix -> 
     Σ ;;; Γ |- tFix mfix n ▹ decl.(dtype)
 
 | infer_CoFix mfix n decl :
     cofix_guard Σ Γ mfix ->
     nth_error mfix n = Some decl ->
-    All_local_env (lift_sorting checking infering_sort Σ) Γ ->
-    All (fun d => {s & Σ ;;; Γ |- d.(dtype) ▹□ s}) mfix ->
+    All (fun d => {s & Σ ;;; Γ |- d.(dtype) ▸□ s}) mfix ->
     All (fun d => Σ ;;; Γ ,,, fix_context mfix |- d.(dbody) ◃ lift0 #|fix_context mfix| d.(dtype)) mfix ->
     wf_cofixpoint Σ.1 mfix ->
     Σ ;;; Γ |- tCoFix mfix n ▹ decl.(dtype)
@@ -153,120 +124,114 @@ with infering_sort `{checker_flags} (Σ : global_env_ext) (Γ : context) : term 
 | infer_sort_Sort t T u:
   Σ ;;; Γ |- t ▹ T ->
   Σ ;;; Γ |- T --> tSort u ->
-  wf_universe Σ u ->
-  Σ ;;; Γ |- t ▹□ u
+  Σ ;;; Γ |- t ▸□ u
 
 with infering_prod `{checker_flags} (Σ : global_env_ext) (Γ : context) : term -> aname -> term -> term -> Type :=
-| infer_prod_Prod t T na A B s:
+| infer_prod_Prod t T na A B:
   Σ ;;; Γ |- t ▹ T ->
   Σ ;;; Γ |- T --> tProd na A B ->
-  Σ ;;; Γ |- tProd na A B ▹□ s ->
-  Σ ;;; Γ |- t ▹Π (na,A,B)
+  Σ ;;; Γ |- t ▸Π (na,A,B)
 
 with infering_indu `{checker_flags} (Σ : global_env_ext) (Γ : context) : inductive -> term -> Instance.t -> list term -> Type :=
-| infer_ind_Ind ind t T u args s:
+| infer_ind_Ind ind t T u args:
   Σ ;;; Γ |- t ▹ T ->
   Σ ;;; Γ |- T --> mkApps (tInd ind u) args ->
-  Σ ;;; Γ |- mkApps (tInd ind u) args ▹□ s ->
-  Σ ;;; Γ |- t ▹{ind} (u,args)
+  Σ ;;; Γ |- t ▸{ind} (u,args)
 
 with checking `{checker_flags} (Σ : global_env_ext) (Γ : context) : term -> term -> Type :=
-| check_Cons t T T' s:
+| check_Cons t T T':
   Σ ;;; Γ |- t ▹ T ->
-  Σ ;;; Γ |- T' ▹□ s ->
   Σ ;;; Γ |- T <= T' ->
   Σ ;;; Γ |- t ◃ T'
 
 where " Σ ;;; Γ |- t ▹ T " := (@infering _ Σ Γ t T) : type_scope
-and " Σ ;;; Γ |- t ▹□ u " := (@infering_sort _ Σ Γ t u) : type_scope
-and " Σ ;;; Γ |- t ▹Π ( na , A , B ) " := (@infering_prod _ Σ Γ t na A B) : type_scope
-and " Σ ;;; Γ |- t ▹{ ind } ( u , args ) " := (@infering_indu _ Σ Γ ind t u args) : type_scope
+and " Σ ;;; Γ |- t ▸□ u " := (@infering_sort _ Σ Γ t u) : type_scope
+and " Σ ;;; Γ |- t ▸Π ( na , A , B ) " := (@infering_prod _ Σ Γ t na A B) : type_scope
+and " Σ ;;; Γ |- t ▸{ ind } ( u , args ) " := (@infering_indu _ Σ Γ ind t u args) : type_scope
 and " Σ ;;; Γ |- t ◃ T " := (@checking _ Σ Γ t T) : type_scope.
 
 Notation wf_local_bd Σ Γ := (All_local_env (lift_sorting checking infering_sort Σ) Γ).
 
-Definition tybranches_bd {cf} Σ Γ ci mdecl idecl p ps ptm n ctors brs :=
-   All2i
-  (fun (i : nat) (cdecl : constructor_body) (br : branch term) =>
-   let brctxty := case_branch_type ci mdecl idecl p br ptm i cdecl in
-   (wf_local_bd Σ (Γ ,,, br.(bcontext)) × 
-    conv_context Σ (Γ ,,, br.(bcontext)) (Γ ,,, brctxty.1)) ×
-   (Σ;;; Γ,,, brctxty.1 |- brctxty.2 ◃ tSort ps
-    × Σ;;; Γ,,, brctxty.1 |- bbody br ◃ brctxty.2)) n ctors brs.
+(** ** Typechecking of global environments, using BDEnvironment to separte typing into checking and sorting *)
 
-Fixpoint wf_local_size_bd `{checker_flags} Σ
-  (sorting_size : forall Σ' Γ t s, Σ' ;;; Γ |- t ▹□ s -> size)
-  (checking_size : forall Σ' Γ t T, Σ' ;;; Γ |- t ◃ T -> size)
-  Γ (w : wf_local_bd Σ Γ) : size :=
-  match w with
-  | localenv_nil => 0
+(* Module BDTypingDef <: Typing PCUICTerm PCUICEnvironment BDEnvTyping.
 
-  | localenv_cons_abs Γ na t wfΓ tty =>
-    sorting_size _ _ t _ (projT2 tty) + wf_local_size_bd Σ sorting_size checking_size _ wfΓ
+  Definition ind_guard := ind_guard.
+  Definition checking `{checker_flags} := checking.
+  Definition sorting `{checker_flags} := infering_sort.
+  Definition wf_universe := @wf_universe.
+  Definition conv := @conv.
+  Definition cumul := @cumul.
+  Definition smash_context := smash_context.
+  Definition expand_lets := expand_lets.
+  Definition extended_subst := extended_subst.
+  Definition expand_lets_ctx := expand_lets_ctx.
+  Definition lift_context := lift_context.
+  Definition subst_context := subst_context.
+  Definition subst_telescope := subst_telescope.
+  Definition subst_instance_context := subst_instance_context.
+  Definition subst_instance_constr := subst_instance_constr.
+  Definition subst := subst.
+  Definition lift := lift.
+  Definition inds := inds. 
+  Definition noccur_between := noccur_between. 
+  Definition closedn := closedn.
+  Definition destArity := destArity [].
 
-  | localenv_cons_def Γ na b t wfΓ tty tty' =>
-    (sorting_size _ _ t _ (projT2 tty)) + (checking_size _ _ b t tty') + wf_local_size_bd  Σ sorting_size checking_size _ wfΓ
-  end.
+End BDTypingDef.
 
-Definition branches_size_bd {cf} {Σ Γ ci mdecl idecl p ps ptm brs}
-   (sorting_size : forall Σ Γ t s, Σ ;;; Γ |- t ▹□ s -> size)
-   (checking_size : forall Σ Γ t T, Σ ;;; Γ |- t ◃ T -> size)
-  {n ctors}
-  (a : tybranches_bd Σ Γ ci mdecl idecl p ps ptm n ctors brs) : size :=
-  (all2i_size _ (fun i x y p => 
-    Nat.max (wf_local_size_bd _ sorting_size checking_size _ p.1.1)
-      (Nat.max (checking_size _ _ _ _ p.2.1) (checking_size _ _ _ _ p.2.2))) a).
+Module BDDeclarationTyping :=
+  DeclarationTyping
+    PCUICTerm
+    PCUICEnvironment
+    BDEnvTyping
+    BDTypingDef
+    BDLookup.
+Include BDDeclarationTyping. *)
 
 Fixpoint infering_size `{checker_flags} {Σ Γ t T} (d : Σ ;;; Γ |- t ▹ T) {struct d} : size
-with infering_sort_size `{checker_flags} {Σ Γ t u} (d : Σ ;;; Γ |- t ▹□ u) {struct d} : size
-with infering_prod_size `{checker_flags} {Σ Γ t na A B} (d : Σ ;;; Γ |- t ▹Π (na, A,B)) {struct d} : size
-with infering_indu_size `{checker_flags} {Σ Γ ind t ui args} (d : Σ ;;; Γ |- t ▹{ind} (ui,args)) {struct d} : size
+with infering_sort_size `{checker_flags} {Σ Γ t u} (d : Σ ;;; Γ |- t ▸□ u) {struct d} : size
+with infering_prod_size `{checker_flags} {Σ Γ t na A B} (d : Σ ;;; Γ |- t ▸Π (na, A,B)) {struct d} : size
+with infering_indu_size `{checker_flags} {Σ Γ ind t ui args} (d : Σ ;;; Γ |- t ▸{ind} (ui,args)) {struct d} : size
 with checking_size `{checker_flags} {Σ Γ t T} (d : Σ ;;; Γ |- t ◃ T) {struct d} : size.
 Proof.
   all: destruct d ;
-    repeat lazymatch goal with
+    repeat match goal with
           | H : infering _ _ _ _ |- _ => apply infering_size in H
           | H : infering_sort _ _ _ _ |- _ => apply infering_sort_size in H
           | H : infering_prod _ _ _ _ _ _ |- _ => apply infering_prod_size in H
           | H : infering_indu _ _ _ _ _ _ |- _ => apply infering_indu_size in H 
           | H : checking _ _ _ _ |- _ => apply checking_size in H
-          | H : wf_local_bd _ _ |- _ => apply (wf_local_size_bd _ (infering_sort_size _) (checking_size _)) in H
-    end;
-    lazymatch goal with
-    | H : All2i _ _ _ _ |- _ => idtac
+          | H : wf_local _ _ |- _ => apply (wf_local_size _ (checking_size _) (infering_sort_size _)) in H
+          end ;
+    match goal with
+    | H : All2 _ _ _ |- _ => idtac
     | H : All _ _ |- _ => idtac
     | H1 : size, H2 : size, H3 : size |- _ => exact (S (H1 + H2 + H3))
     | H1 : size, H2 : size |- _ => exact (S (H1 + H2))
     | H1 : size |- _  => exact (S H1)
+    | |- _ => exact 1
     end.
     - exact (S (i + c0 + (all2_size _ 
-                                        (fun x y p => (infering_sort_size _ _ _ _ _ (fst (snd p)))
-                                                      + (checking_size _ _ _ _ _ (snd (snd p)))) a))).
-    - exact (S (a + (all_size _ (fun d p => infering_sort_size _ _ _ _ _ p.π2) a0) +
-               (all_size _ (fun x p => checking_size _ _ _ _ _ p.1) a1))).
-    - exact (S (a + (all_size _ (fun d p => infering_sort_size _ _ _ _ _ p.π2) a0) +
-               (all_size _ (fun x => checking_size _ _ _ _ _) a1))).
+                                      (fun x y p => checking_size _ _ _ _ _ (snd p))) a)).
+    - exact (S (all_size _ (fun d p => infering_sort_size _ _ _ _ _ p.π2) a) +
+               (all_size _ (fun x p => checking_size _ _ _ _ _ p) a0)).
+    - exact (S (all_size _ (fun d p => infering_sort_size _ _ _ _ _ p.π2) a) +
+               (all_size _ (fun x => checking_size _ _ _ _ _) a0)).
   Defined.
-
-(* Definition wfarity_size `{checker_flags} {Σ Γ T} (d : isWfArity_sorting checking infering_sort Σ Γ T) : size.
-Proof.
-  destruct d as (ctx & u & e & wf).
-  exact (wf_local_size Σ (@checking_size _) (@infering_sort_size _) _ wf).
-Defined. *)
 
 Fixpoint infering_size_pos `{checker_flags} {Σ Γ t T} (d : Σ ;;; Γ |- t ▹ T)
   : infering_size d > 0
-with infering_sort_size_pos `{checker_flags} {Σ Γ t u} (d : Σ ;;; Γ |- t ▹□ u) {struct d}
+with infering_sort_size_pos `{checker_flags} {Σ Γ t u} (d : Σ ;;; Γ |- t ▸□ u) {struct d}
   : infering_sort_size d > 0
-with infering_prod_size_pos `{checker_flags} {Σ Γ t na A B} (d : Σ ;;; Γ |- t ▹Π (na,A,B)) {struct d}
+with infering_prod_size_pos `{checker_flags} {Σ Γ t na A B} (d : Σ ;;; Γ |- t ▸Π (na,A,B)) {struct d}
   : infering_prod_size d > 0
-with infering_indu_size_pos `{checker_flags} {Σ Γ t ind ui args} (d : Σ ;;; Γ |- t ▹{ind} (ui,args)) {struct d}
+with infering_indu_size_pos `{checker_flags} {Σ Γ t ind ui args} (d : Σ ;;; Γ |- t ▸{ind} (ui,args)) {struct d}
   : infering_indu_size d > 0
 with checking_size_pos `{checker_flags} {Σ Γ t T} (d : Σ ;;; Γ |- t ◃ T) {struct d}
   : checking_size d > 0.
 Proof.
   all: destruct d ; cbn.
-  all: match goal with | H: _ + _ |- _ => destruct H as [[? [? []]]|[]] | _ => idtac end.
   all: lia.
 Qed.
 
@@ -279,66 +244,28 @@ Fixpoint globenv_size (Σ : global_env) : size :=
 
 Arguments lexprod [A B].
 
-Definition wf `{checker_flags} := Forall_decls_sorting checking infering_sort.
-Definition wf_ext `{checker_flags} := on_global_env_ext checking infering_sort.
+Section BidirectionalInduction.
 
-Lemma wf_ext_wf {cf:checker_flags} Σ : wf_ext Σ -> wf Σ.
-Proof. intro H; apply H. Qed.
+#[local] Notation wfl_size := (All_local_env_sorting_size _ _ (@checking_size _) (@infering_sort_size _) _ _).
 
-Hint Resolve wf_ext_wf : core.
-
-Lemma wf_ext_consistent {cf:checker_flags} Σ :
-  wf_ext Σ -> consistent Σ.
-Proof.
-  intros [? [? [? [? ?]]]]; assumption.
-Qed.
-
-Hint Resolve wf_ext_consistent : core.
-
-Lemma wf_local_app `{checker_flags} Σ (Γ Γ' : context) : wf_local Σ (Γ ,,, Γ') -> wf_local Σ Γ.
-Proof.
-  induction Γ'. auto.
-  simpl. intros H'; inv H'; eauto.
-Defined.
-Hint Resolve wf_local_app : wf.
-
-Fixpoint infering_wf_local `{checker_flags} {Σ Γ t T} (d : Σ ;;; Γ |- t ▹ T)
-  : wf_local Σ Γ
-with infering_sort_wf_local `{checker_flags} {Σ Γ t u} (d : Σ ;;; Γ |- t ▹□ u) {struct d}
-  : wf_local Σ Γ
-with infering_prod_wf_local `{checker_flags} {Σ Γ t na A B} (d : Σ ;;; Γ |- t ▹Π (na,A,B)) {struct d}
-  : wf_local Σ Γ
-with infering_indu_wf_local `{checker_flags} {Σ Γ t ind ui args} (d : Σ ;;; Γ |- t ▹{ind} (ui,args)) {struct d}
-  : wf_local Σ Γ
-with checking_wf_local `{checker_flags} {Σ Γ t T} (d : Σ ;;; Γ |- t ◃ T) {struct d}
-  : wf_local Σ Γ.
-Proof.
-  all: destruct d ; eauto using wf_local_app.
-Defined.
-Hint Resolve typing_wf_local : wf.
-
-Section TypingInduction.
-
-#[local] Notation wfl_size := (wf_local_size _ (@checking_size _) (@infering_sort_size _) _).
-
-  Context (Pcheck : global_env_ext -> context -> term -> term -> Type).
-  Context (Pinfer : global_env_ext -> context -> term -> term -> Type).
-  Context (Psort : global_env_ext -> context -> term -> Universe.t -> Type).
-  Context (Pprod : global_env_ext -> context -> term -> aname -> term -> term -> Type).
-  Context (Pind : global_env_ext -> context -> inductive -> term -> Instance.t -> list term -> Type).
-  Context (PΓ : forall `{checker_flags} Σ Γ, wf_local Σ Γ -> Type).
-  Arguments PΓ {_}.
+  Context `{cf : checker_flags}.
+  Context (Σ : global_env_ext).
+  Context (wfΣ : wf Σ).
+  Context (Pcheck : context -> term -> term -> Type).
+  Context (Pinfer : context -> term -> term -> Type).
+  Context (Psort : context -> term -> Universe.t -> Type).
+  Context (Pprod : context -> term -> aname -> term -> term -> Type).
+  Context (Pind : context -> inductive -> term -> Instance.t -> list term -> Type).
+  Context (PΓ : forall Γ, wf_local_bd Σ Γ -> Type).
 
 (* This is what we wish to prove with our mutual induction principle, note how also global environment and local context are built-in *)
-  Definition env_prop `{checker_flags} :=
-    forall Σ (wfΣ : wf Σ.1),
-    (Forall_decls_sorting Pcheck Psort Σ.1) ×
-    (forall Γ (wfΓ : wf_local Σ Γ), PΓ Σ Γ wfΓ) ×
-    (forall Γ t T, Σ ;;; Γ |- t ◃ T -> Pcheck Σ Γ t T) ×
-    (forall Γ t T, Σ ;;; Γ |- t ▹ T -> Pinfer Σ Γ t T) ×
-    (forall Γ t u, Σ ;;; Γ |- t ▹□ u -> Psort Σ Γ t u) ×
-    (forall Γ t na A B, Σ ;;; Γ |- t ▹Π (na,A,B) -> Pprod Σ Γ t na A B) ×
-    (forall Γ ind t u args, Σ ;;; Γ |- t ▹{ind} (u,args) -> Pind Σ Γ ind t u args).
+  Definition env_prop_bd :=
+    (forall Γ wfΓ, PΓ Γ wfΓ) ×
+    (forall Γ t T, Σ ;;; Γ |- t ◃ T -> Pcheck Γ t T) ×
+    (forall Γ t T, Σ ;;; Γ |- t ▹ T -> Pinfer Γ t T) ×
+    (forall Γ t u, Σ ;;; Γ |- t ▸□ u -> Psort Γ t u) ×
+    (forall Γ t na A B, Σ ;;; Γ |- t ▸Π (na,A,B) -> Pprod Γ t na A B) ×
+    (forall Γ ind t u args, Σ ;;; Γ |- t ▸{ind} (u,args) -> Pind Γ ind t u args).
 
   Derive Signature for All_local_env.
 
@@ -347,459 +274,248 @@ Section TypingInduction.
   Derive NoConfusion for list.
   Derive NoConfusion for All_local_env.
 
-  Lemma size_wf_local_app `{checker_flags} {Σ} (Γ Γ' : context) (Hwf : wf_local Σ (Γ ,,, Γ')) :
-    wfl_size (wf_local_app _ _ _ Hwf) <=
-    wfl_size Hwf.
-  Proof.
-    induction Γ' in Γ, Hwf |- *; try lia. simpl. lia.
-    depelim Hwf.
-    - inversion t0. subst. noconf X. simpl. unfold eq_rect_r. simpl. specialize (IHΓ' _ Hwf). lia.
-    - inversion t0. subst. noconf X. specialize (IHΓ' _ Hwf). simpl. unfold eq_rect_r. simpl. lia.
-  Qed.
-
-  Fixpoint infering_wf_local_size `{checker_flags} {Σ Γ t T} (d : Σ ;;; Γ |- t ▹ T)
-    : wfl_size (infering_wf_local d) < infering_size d
-  with infering_sort_wf_local_size `{checker_flags} {Σ Γ t u} (d : Σ ;;; Γ |- t ▹□ u) {struct d}
-    : wfl_size (infering_sort_wf_local d) < infering_sort_size d
-  with infering_prod_wf_local_size `{checker_flags} {Σ Γ t na A B} (d : Σ ;;; Γ |- t ▹Π (na,A,B)) {struct d}
-    : wfl_size (infering_prod_wf_local d) < infering_prod_size d
-  with infering_indu_wf_local_size `{checker_flags} {Σ Γ t ind ui args} (d : Σ ;;; Γ |- t ▹{ind} (ui,args)) {struct d}
-    : wfl_size (infering_indu_wf_local d) < infering_indu_size d
-  with checking_wf_local_size `{checker_flags} {Σ Γ t T} (d : Σ ;;; Γ |- t ◃ T) {struct d}
-  : wfl_size (checking_wf_local d) < checking_size d.
-  Proof.
-    all: destruct d ; simpl.
-    all: match goal with | H: _ + _ |- _ => destruct H as [[? [? []]]|[]] | _ => idtac end.
-    all: match goal with
-      | |- context [infering_wf_local ?i] =>
-            specialize (infering_wf_local_size _ _ _ _ _ i)
-      | |- context [infering_sort_wf_local ?i] =>
-            specialize (infering_sort_wf_local_size _ _ _ _ _ i)
-      | |- context [infering_prod_wf_local ?i] =>
-            specialize (infering_prod_wf_local_size _ _ _ _ _ _ _ i)
-      | |- context [infering_indu_wf_local ?i] =>
-            specialize (infering_indu_wf_local_size _ _ _ _ _ _ _ i)
-      | |- context [checking_wf_local ?i] =>
-            specialize (checking_wf_local_size _ _ _ _ _ i)
-      | _ => idtac
-    end.
-    all: lia.
-  Qed.
-
- (*  Lemma isWfArity_sort `{checker_flags} {Σ Γ} (wfΓ : wf_local Σ Γ) u : isWfArity_sorting checking infering_sort Σ Γ (tSort u).
-  Proof.
-    red. exists []. exists u.
-    split.
-    1: by rewrite /destArity /=.
-    assumption.
-  Defined. *)
-
   Derive Signature for Alli.
 
   (** *** To prove the needed induction principle, we unite all possible typing judgments in a big sum type,
           on which we define a suitable notion of size, wrt. which we perform well-founded induction
   *)
 
-  Inductive typing_sum `{checker_flags} Σ (wfΣ : wf Σ.1) : Type :=
-    | env_cons : typing_sum Σ wfΣ
-    | context_cons : forall (Γ : context) (wfΓ : wf_local Σ Γ), typing_sum Σ wfΣ
-    | check_cons : forall (Γ : context) T t, Σ ;;; Γ |- t ◃ T -> typing_sum Σ wfΣ
-    | inf_cons : forall (Γ : context) T t, Σ ;;; Γ |- t ▹ T -> typing_sum Σ wfΣ
-    | sort_cons : forall (Γ : context) t u, Σ ;;; Γ |- t ▹□ u -> typing_sum Σ wfΣ
-    | prod_cons : forall (Γ : context) t na A B, Σ ;;; Γ |- t ▹Π (na,A,B) -> typing_sum Σ wfΣ
-    | ind_cons : forall (Γ : context) ind t u args,
-        Σ ;;; Γ |- t ▹{ind} (u,args) -> typing_sum Σ wfΣ.
+  Inductive typing_sum : Type :=
+    | context_cons : forall (Γ : context) (wfΓ : wf_local_bd Σ Γ), typing_sum
+    | check_cons : forall (Γ : context) T t, Σ ;;; Γ |- t ◃ T -> typing_sum
+    | inf_cons : forall (Γ : context) T t, Σ ;;; Γ |- t ▹ T -> typing_sum
+    | sort_cons : forall (Γ : context) t u, Σ ;;; Γ |- t ▸□ u -> typing_sum
+    | prod_cons : forall (Γ : context) t na A B, Σ ;;; Γ |- t ▸Π (na,A,B) -> typing_sum
+    | ind_cons : forall (Γ : context) ind t u args, Σ ;;; Γ |- t ▸{ind} (u,args) -> typing_sum.
 
-  Definition typing_sum_size `{checker_flags} {Σ} {wfΣ : wf Σ.1} (d : typing_sum Σ wfΣ) :=
+  Definition typing_sum_size (d : typing_sum) :=
   match d with
-    | env_cons => 0
     | context_cons Γ wfΓ => wfl_size wfΓ
-    | check_cons Γ _ _ d => (checking_size d)
-    | inf_cons Γ _ _ d => (infering_size d)
-    | sort_cons Γ _ _ d => (infering_sort_size d)
-    | prod_cons Γ _ _ _ _ d => (infering_prod_size d)
-    | ind_cons Γ _ _ _ _ d => (infering_indu_size d)
+    | check_cons _ _ _ d => (checking_size d)
+    | inf_cons _ _ _ d => (infering_size d)
+    | sort_cons _ _ _ d => (infering_sort_size d)
+    | prod_cons _ _ _ _ _ d => (infering_prod_size d)
+    | ind_cons _ _ _ _ _ d => (infering_indu_size d)
   end.
-  
-  Definition Ptyping_sum `{checker_flags} {Σ wfΣ} (d : typing_sum Σ wfΣ) :=
+
+  Definition Ptyping_sum (d : typing_sum) :=
   match d with
-    | env_cons => Forall_decls_sorting Pcheck Psort Σ.1
-    | context_cons Γ wfΓ => PΓ Σ Γ wfΓ
-    | check_cons Γ T t _ => Pcheck Σ Γ t T
-    | inf_cons Γ T t _ => Pinfer Σ Γ t T
-    | sort_cons Γ T u _ => Psort Σ Γ T u
-    | prod_cons Γ T na A B _ => Pprod Σ Γ T na A B
-    | ind_cons Γ ind T u args _ => Pind Σ Γ ind T u args
+    | context_cons Γ wfΓ => PΓ Γ wfΓ
+    | check_cons Γ T t _ => Pcheck Γ t T
+    | inf_cons Γ T t _ => Pinfer Γ t T
+    | sort_cons Γ T u _ => Psort Γ T u
+    | prod_cons Γ T na A B _ => Pprod Γ T na A B
+    | ind_cons Γ ind T u args _ => Pind Γ ind T u args
   end.
 
   Ltac applyIH := match goal with
-    | IH : forall _ _ d', _ -> Ptyping_sum d' |- Forall_decls_sorting Pcheck Psort _ =>
-          unshelve eapply (IH _ _ (env_cons _ _))
-    | IH : forall Σ' wfΣ' d', _ -> Ptyping_sum d' |- PΓ _ ?Γ ?wfΓ =>
-          unshelve eapply (IH _ _ (context_cons _ _ Γ wfΓ))
-    | IH : forall Σ' wfΣ' d', _ -> Ptyping_sum d' |- Pcheck _ ?Γ ?t ?T =>
-          unshelve eapply (IH _ _ (check_cons _ _ Γ T t _))
-    | IH : forall Σ' wfΣ' d', _ -> Ptyping_sum d' |- Pinfer _ ?Γ ?t ?T =>
-          unshelve eapply (IH _ _ (inf_cons _ _ Γ T t _))
-    | IH : forall Σ' wfΣ' d', _ -> Ptyping_sum d'|- Psort _ ?Γ ?t ?u =>
-          unshelve eapply (IH _ _ (sort_cons _ _ Γ t u _))
-    | IH : forall Σ' wfΣ' d', _ -> Ptyping_sum d' |- Pprod _ ?Γ ?t ?na ?A ?B =>
-          unshelve eapply (IH _ _ (prod_cons _ _ Γ t na A B _))
-    | IH : forall Σ' wfΣ' d', _ -> Ptyping_sum d' |- Pind _ ?Γ ?ind ?t ?u ?args =>
-          unshelve eapply (IH _ _ (ind_cons _ _ Γ ind t u args _))
+    | IH : forall d', _ -> Ptyping_sum d' |- PΓ ?Γ ?wfΓ =>
+      unshelve eapply (IH (context_cons Γ wfΓ))
+    | IH : forall d', _ -> Ptyping_sum d' |- Pcheck ?Γ ?t ?T =>
+      unshelve eapply (IH (check_cons Γ T t _))
+    | IH : forall d', _ -> Ptyping_sum d' |- Pinfer ?Γ ?t ?T =>
+      unshelve eapply (IH (inf_cons Γ T t _))
+    | IH : forall d', _ -> Ptyping_sum d'|- Psort ?Γ ?t ?u =>
+      unshelve eapply (IH (sort_cons Γ t u _))
+    | IH : forall d', _ -> Ptyping_sum d' |- Pprod ?Γ ?t ?na ?A ?B =>
+      unshelve eapply (IH (prod_cons Γ t na A B _))
+    | IH : forall d', _ -> Ptyping_sum d' |- Pind ?Γ ?ind ?t ?u ?args =>
+      unshelve eapply (IH (ind_cons Γ ind t u args _))
     end ;
     match goal with
-(*     | |- isWfArity _ _ _ (tSort _) => apply isWfArity_sort ; try assumption ; try (by constructor) *)
     | |- dlexprod _ _ _ _ => constructor ; simpl ; lia
     | |- dlexprod _ _ _ _ =>
-            constructor 2 ; simpl ;
-            (match goal with | |- dlexprod _ _ (?x1;_) (?y1;_) => replace x1 with y1 by lia end ; constructor 2) ||
-            constructor ; try lia
+            constructor 2 ; simpl ; try lia
     | _ => assumption
     | _ => simpl ; lia
     | _ => idtac
     end.
 
-  Lemma typing_ind_env `{cf : checker_flags} :
-    let Pdecl_check := fun Σ Γ wfΓ t T tyT => Pcheck Σ Γ t T in
-    let Pdecl_sort := fun Σ Γ wfΓ t u tyT => Psort Σ Γ t u in
+  Lemma bidir_ind_env :
+    let Pdecl_check := fun Σ Γ wfΓ t T tyT => Pcheck Γ t T in
+    let Pdecl_sort := fun Σ Γ wfΓ t u tyT => Psort Γ t u in
 
-    (forall Σ (wfΣ : wf Σ.1) (PΣ : Forall_decls_sorting Pcheck Psort Σ.1)
-      (Γ : context) (wfΓ : wf_local Σ Γ), 
-      All_local_env_over_sorting checking infering_sort Pdecl_check Pdecl_sort Σ Γ wfΓ -> PΓ Σ Γ wfΓ) ->
+    (forall (Γ : context) (wfΓ : wf_local_bd Σ Γ), 
+      All_local_env_over_sorting checking infering_sort Pdecl_check Pdecl_sort Σ Γ wfΓ -> PΓ Γ wfΓ) ->
 
-    (forall Σ (wfΣ : wf Σ.1) (PΣ : Forall_decls_sorting Pcheck Psort Σ.1)
-      (Γ : context) (wfΓ : wf_local Σ Γ) (n : nat) decl,
-      PΓ Σ Γ wfΓ ->
+    (forall (Γ : context) (n : nat) decl,
       nth_error Γ n = Some decl ->
-      Pinfer Σ Γ (tRel n) (lift0 (S n) decl.(decl_type))) ->
+      Pinfer Γ (tRel n) (lift0 (S n) decl.(decl_type))) ->
 
-    (forall Σ (wfΣ : wf Σ.1)(PΣ : Forall_decls_sorting Pcheck Psort Σ.1)
-      (Γ : context) (wfΓ : wf_local Σ Γ) (s : Universe.t),
-      PΓ Σ Γ wfΓ ->
+    (forall (Γ : context) (s : Universe.t),
       wf_universe Σ s->
-      Pinfer Σ Γ (tSort s) (tSort (Universe.super s))) ->
+      Pinfer Γ (tSort s) (tSort (Universe.super s))) ->
 
-    (forall Σ (wfΣ : wf Σ.1) (PΣ : Forall_decls_sorting Pcheck Psort Σ.1)
-      (Γ : context) (wfΓ : wf_local Σ Γ) (n : aname) (t b : term) (s1 s2 : Universe.t),
-      PΓ Σ Γ wfΓ ->
-      Σ ;;; Γ |- t ▹□ s1 ->
-      Psort Σ Γ t s1 ->
-      Σ ;;; Γ,, vass n t |- b ▹□ s2 ->
-      Psort Σ (Γ,, vass n t) b s2 ->
-      Pinfer Σ Γ (tProd n t b) (tSort (Universe.sort_of_product s1 s2))) ->
+    (forall (Γ : context) (n : aname) (t b : term) (s1 s2 : Universe.t),
+      Σ ;;; Γ |- t ▸□ s1 ->
+      Psort Γ t s1 ->
+      Σ ;;; Γ,, vass n t |- b ▸□ s2 ->
+      Psort (Γ,, vass n t) b s2 ->
+      Pinfer Γ (tProd n t b) (tSort (Universe.sort_of_product s1 s2))) ->
 
-    (forall Σ (wfΣ : wf Σ.1) (PΣ : Forall_decls_sorting Pcheck Psort Σ.1)
-      (Γ : context) (wfΓ : wf_local Σ Γ) (n : aname) (t b : term) (s : Universe.t) (bty : term),
-      PΓ Σ Γ wfΓ ->
-      Σ ;;; Γ |- t ▹□ s ->
-      Psort Σ Γ t s ->
-      Σ ;;; Γ,, vass n t |- b ▹ bty -> Pinfer Σ (Γ,, vass n t) b bty ->
-      Pinfer Σ Γ (tLambda n t b) (tProd n t bty)) ->
+    (forall (Γ : context) (n : aname) (t b : term) (s : Universe.t) (bty : term),
+      Σ ;;; Γ |- t ▸□ s ->
+      Psort Γ t s ->
+      Σ ;;; Γ,, vass n t |- b ▹ bty ->
+      Pinfer (Γ,, vass n t) b bty ->
+      Pinfer Γ (tLambda n t b) (tProd n t bty)) ->
 
-    (forall Σ (wfΣ : wf Σ.1) (PΣ : Forall_decls_sorting Pcheck Psort Σ.1)
-      (Γ : context) (wfΓ : wf_local Σ Γ) (n : aname) (b B t : term) (s : Universe.t) (A : term),
-      PΓ Σ Γ wfΓ ->
-      Σ ;;; Γ |- B ▹□ s ->
-      Psort Σ Γ B s ->
+    (forall (Γ : context) (n : aname) (b B t : term) (s : Universe.t) (A : term),
+      Σ ;;; Γ |- B ▸□ s ->
+      Psort Γ B s ->
       Σ ;;; Γ |- b ◃ B ->
-      Pcheck Σ Γ b B ->
+      Pcheck Γ b B ->
       Σ ;;; Γ,, vdef n b B |- t ▹ A ->
-      Pinfer Σ (Γ,, vdef n b B) t A -> Pinfer Σ Γ (tLetIn n b B t) (tLetIn n b B A)) ->
+      Pinfer (Γ,, vdef n b B) t A ->
+      Pinfer Γ (tLetIn n b B t) (tLetIn n b B A)) ->
 
-    (forall Σ (wfΣ : wf Σ.1) (PΣ : Forall_decls_sorting Pcheck Psort Σ.1)
-      (Γ : context) (wfΓ : wf_local Σ Γ) (t : term) na A B u,
-      PΓ Σ Γ wfΓ ->
-      Σ ;;; Γ |- t ▹Π (na, A, B) -> Pprod Σ Γ t na A B ->
-      Σ ;;; Γ |- u ◃ A -> Pcheck Σ Γ u A ->
-      Pinfer Σ Γ (tApp t u) (subst10 u B)) ->
+    (forall (Γ : context) (t : term) na A B u,
+      Σ ;;; Γ |- t ▸Π (na, A, B) ->
+      Pprod Γ t na A B ->
+      Σ ;;; Γ |- u ◃ A ->
+      Pcheck Γ u A ->
+      Pinfer Γ (tApp t u) (subst10 u B)) ->
 
-    (forall Σ (wfΣ : wf Σ.1) (PΣ : Forall_decls_sorting Pcheck Psort Σ.1)
-      (Γ : context) (wfΓ : wf_local Σ Γ) (cst : kername) u (decl : constant_body),
-      PΓ Σ Γ wfΓ ->
-      Forall_decls_sorting Pcheck Psort Σ.1 ->
+    (forall (Γ : context) (cst : kername) u (decl : constant_body),
       declared_constant Σ.1 cst decl ->
       consistent_instance_ext Σ decl.(cst_universes) u ->
-      Pinfer Σ Γ (tConst cst u) (subst_instance_constr u (cst_type decl))) ->
+      Pinfer Γ (tConst cst u) (subst_instance_constr u (cst_type decl))) ->
 
-    (forall Σ (wfΣ : wf Σ.1) (PΣ : Forall_decls_sorting Pcheck Psort Σ.1)
-      (Γ : context) (wfΓ : wf_local Σ Γ) (ind : inductive) u mdecl idecl,
-      PΓ Σ Γ wfΓ ->
-      Forall_decls_sorting Pcheck Psort Σ.1 ->
+    (forall (Γ : context) (ind : inductive) u mdecl idecl,
       declared_inductive Σ.1 mdecl ind idecl ->
       consistent_instance_ext Σ mdecl.(ind_universes) u ->
-      Pinfer Σ Γ (tInd ind u) (subst_instance_constr u (ind_type idecl))) ->
+      Pinfer Γ (tInd ind u) (subst_instance_constr u (ind_type idecl))) ->
 
-    (forall Σ (wfΣ : wf Σ.1) (PΣ : Forall_decls_sorting Pcheck Psort Σ.1)
-      (Γ : context) (wfΓ : wf_local Σ Γ) (ind : inductive) (i : nat) u
+    (forall (Γ : context) (ind : inductive) (i : nat) u
       mdecl idecl cdecl,
-      PΓ Σ Γ wfΓ ->
-      Forall_decls_sorting Pcheck Psort Σ.1 ->
       declared_constructor Σ.1 mdecl idecl (ind, i) cdecl ->
       consistent_instance_ext Σ mdecl.(ind_universes) u ->
-      Pinfer Σ Γ (tConstruct ind i u)
+      Pinfer Γ (tConstruct ind i u)
         (type_of_constructor mdecl cdecl (ind, i) u)) ->
 
-    (forall Σ (wfΣ : wf Σ.1) (PΣ : Forall_decls_sorting Pcheck Psort Σ.1)
-      (Γ : context) (wfΓ : wf_local Σ Γ) (ind : inductive) u (npar : nat)
+    (forall (Γ : context) (ind : inductive) u (npar : nat)
       (p c : term) (brs : list (nat * term)) (args : list term)
       (mdecl : mutual_inductive_body) (idecl : one_inductive_body)
       (isdecl : declared_inductive (fst Σ) mdecl ind idecl),
-      PΓ Σ Γ wfΓ ->
-      Forall_decls_sorting Pcheck Psort Σ.1 ->
-      isCoFinite mdecl.(ind_finite) = false ->
-      Σ ;;; Γ |- c ▹{ind} (u,args) ->
-      Pind Σ Γ ind c u args ->
       ind_npars mdecl = npar ->
+      isCoFinite mdecl.(ind_finite) = false ->
+      Σ ;;; Γ |- c ▸{ind} (u,args) ->
+      Pind Γ ind c u args ->
       let params := firstn npar args in
       forall ps pty,
+      wf_universe Σ ps ->
       build_case_predicate_type ind mdecl idecl params u ps = Some pty ->
       Σ ;;; Γ |- p ◃ pty ->
-      Pcheck Σ Γ p pty ->
-      leb_sort_family (universe_family ps) idecl.(ind_kelim) ->
+      Pcheck Γ p pty ->
+      is_allowed_elimination Σ ps (ind_kelim idecl) ->
       forall btys,
       map_option_out (build_branches_type ind mdecl idecl params u p) = Some btys ->
       All2 (fun br bty => (br.1 = bty.1) ×
-                        (Σ ;;; Γ |- bty.2 ▹□ ps) × Psort Σ Γ bty.2 ps ×
-                        (Σ ;;; Γ |- br.2 ◃ bty.2) × Pcheck Σ Γ br.2 bty.2)
+                        (Σ ;;; Γ |- br.2 ◃ bty.2) × Pcheck Γ br.2 bty.2)
             brs btys ->
-      Pinfer Σ Γ (tCase (ind,npar) p c brs) (mkApps p (skipn npar args ++ [c]))) ->
+      Pinfer Γ (tCase (ind,npar) p c brs) (mkApps p (skipn npar args ++ [c]))) ->
 
-    (forall Σ (wfΣ : wf Σ.1) (PΣ : Forall_decls_sorting Pcheck Psort Σ.1)
-      (Γ : context) (wfΓ : wf_local Σ Γ) (p : projection) (c : term) u
+    (forall (Γ : context) (p : projection) (c : term) u
       mdecl idecl pdecl args,
-      PΓ Σ Γ wfΓ ->
-      Forall_decls_sorting Pcheck Psort Σ.1 ->
       declared_projection Σ.1 mdecl idecl p pdecl ->
-      Σ ;;; Γ |- c ▹{fst (fst p)} (u,args) ->
-      Pind Σ Γ (fst (fst p)) c u args ->
+      Σ ;;; Γ |- c ▸{fst (fst p)} (u,args) ->
+      Pind Γ (fst (fst p)) c u args ->
       #|args| = ind_npars mdecl ->
       let ty := snd pdecl in
-      Pinfer Σ Γ (tProj p c) (subst0 (c :: List.rev args) (subst_instance_constr u ty))) ->
+      Pinfer Γ (tProj p c) (subst0 (c :: List.rev args) (subst_instance_constr u ty))) ->
 
-    (forall Σ (wfΣ : wf Σ.1) (PΣ : Forall_decls_sorting Pcheck Psort Σ.1)
-      (Γ : context) (wfΓ : wf_local Σ Γ) (mfix : mfixpoint term) (n : nat) decl,
-      PΓ Σ Γ wfΓ ->
-      fix_guard mfix ->
+    (forall (Γ : context) (mfix : mfixpoint term) (n : nat) decl,
+      fix_guard Σ Γ mfix ->
       nth_error mfix n = Some decl ->
-      All (fun d => {s & (Σ ;;; Γ |- d.(dtype) ▹□ s) × Psort Σ Γ d.(dtype) s}) mfix ->
+      All (fun d => {s & (Σ ;;; Γ |- d.(dtype) ▸□ s) × Psort Γ d.(dtype) s}) mfix ->
       All (fun d => (Σ ;;; Γ ,,, fix_context mfix |- d.(dbody) ◃ lift0 #|fix_context mfix| d.(dtype)) ×
-                (isLambda d.(dbody) = true) ×
-                Pcheck Σ (Γ ,,, fix_context mfix) d.(dbody) (lift0 #|fix_context mfix| d.(dtype))) mfix ->
+                Pcheck (Γ ,,, fix_context mfix) d.(dbody) (lift0 #|fix_context mfix| d.(dtype))) mfix ->
       wf_fixpoint Σ.1 mfix ->
-      Pinfer Σ Γ (tFix mfix n) decl.(dtype)) ->
+      Pinfer Γ (tFix mfix n) decl.(dtype)) ->
     
-    (forall Σ (wfΣ : wf Σ.1) (PΣ : Forall_decls_sorting Pcheck Psort Σ.1)
-      (Γ : context) (wfΓ : wf_local Σ Γ) (mfix : mfixpoint term) (n : nat) decl,
-      PΓ Σ Γ wfΓ ->
-      cofix_guard mfix ->
+    (forall (Γ : context) (mfix : mfixpoint term) (n : nat) decl,
+      cofix_guard Σ Γ mfix ->
       nth_error mfix n = Some decl ->
-      All (fun d => {s & (Σ ;;; Γ |- d.(dtype) ▹□ s) × Psort Σ Γ d.(dtype) s}) mfix ->
+      All (fun d => {s & (Σ ;;; Γ |- d.(dtype) ▸□ s) × Psort Γ d.(dtype) s}) mfix ->
       All (fun d => (Σ ;;; Γ ,,, fix_context mfix |- d.(dbody) ◃ lift0 #|fix_context mfix| d.(dtype)) ×
-                Pcheck Σ (Γ ,,, fix_context mfix) d.(dbody) (lift0 #|fix_context mfix| d.(dtype))) mfix ->
+                Pcheck (Γ ,,, fix_context mfix) d.(dbody) (lift0 #|fix_context mfix| d.(dtype))) mfix ->
       wf_cofixpoint Σ.1 mfix ->
-      Pinfer Σ Γ (tCoFix mfix n) decl.(dtype)) ->
+      Pinfer Γ (tCoFix mfix n) decl.(dtype)) ->
 
-    (forall (Σ : global_env_ext) (wfΣ : wf Σ.1) (PΣ : Forall_decls_sorting Pcheck Psort Σ.1)
-      (Γ : context) (wfΓ : wf_local Σ Γ) (t T : term) (u : Universe.t),
-      PΓ Σ Γ wfΓ ->
+    (forall (Γ : context) (t T : term) (u : Universe.t),
       Σ ;;; Γ |- t ▹ T ->
-      Pinfer Σ Γ t T ->
+      Pinfer Γ t T ->
       Σ ;;; Γ |- T --> tSort u ->
-      wf_universe Σ u ->
-      Psort Σ Γ t u) ->
+      Psort Γ t u) ->
 
-    (forall (Σ : global_env_ext) (wfΣ : wf Σ.1) (PΣ : Forall_decls_sorting Pcheck Psort Σ.1)
-      (Γ : context) (wfΓ : wf_local Σ Γ) (t T : term) (na : aname) (A B : term) (s : Universe.t),
-      PΓ Σ Γ wfΓ ->
+    (forall (Γ : context) (t T : term) (na : aname) (A B : term),
       Σ ;;; Γ |- t ▹ T ->
-      Pinfer Σ Γ t T ->
+      Pinfer Γ t T ->
       Σ ;;; Γ |- T --> tProd na A B ->
-      Σ ;;; Γ |- tProd na A B ▹□ s ->
-      Psort Σ Γ (tProd na A B) s ->
-      Pprod Σ Γ t na A B) ->
+      Pprod Γ t na A B) ->
 
-    (forall (Σ : global_env_ext) (wfΣ : wf Σ.1) (PΣ : Forall_decls_sorting Pcheck Psort Σ.1)
-      (Γ : context) (wfΓ : wf_local Σ Γ) (ind : inductive) (t T : term) (ui : Instance.t)
-      (args : list term) (s : Universe.t),
-      PΓ Σ Γ wfΓ ->
+    (forall (Γ : context) (ind : inductive) (t T : term) (ui : Instance.t)
+      (args : list term),
       Σ ;;; Γ |- t ▹ T ->
-      Pinfer Σ Γ t T ->
+      Pinfer Γ t T ->
       Σ ;;; Γ |- T --> mkApps (tInd ind ui) args ->
-      Σ ;;; Γ |- mkApps (tInd ind ui) args ▹□ s ->
-      Psort Σ Γ (mkApps (tInd ind ui) args) s ->
-      Pind Σ Γ ind t ui args) ->
+      Pind Γ ind t ui args) ->
 
-    (forall (Σ : global_env_ext) (wfΣ : wf Σ.1) (PΣ : Forall_decls_sorting Pcheck Psort Σ.1)
-      (Γ : context) (wfΓ : wf_local Σ Γ) (t T T' : term) (s : Universe.t),
-      PΓ Σ Γ wfΓ ->
+    (forall (Γ : context) (t T T' : term),
       Σ ;;; Γ |- t ▹ T ->
-      Pinfer Σ Γ t T ->
-      Σ ;;; Γ |- T' ▹□ s ->
-      Psort Σ Γ T' s ->
+      Pinfer Γ t T ->
       Σ ;;; Γ |- T <= T' ->
-      Pcheck Σ Γ t T') ->
+      Pcheck Γ t T') ->
       
-    env_prop.
+    env_prop_bd.
   Proof.
     intros Pdecl_check Pdecl_sort HΓ HRel HSort HProd HLambda HLetIn HApp HConst HInd HConstruct HCase
-      HProj HFix HCoFix HiSort HiProd HiInd HCheck ; unfold env_prop.
-    pose (@Fix_F (∑ (Σ : _) (wfΣ : _), typing_sum Σ wfΣ)
-      (dlexprod (precompose lt (fun Σ => globenv_size (fst Σ)))
-        (fun Σ => precompose lt (fun d => typing_sum_size d.π2)))
-      (fun d => Ptyping_sum d.π2.π2)).
+      HProj HFix HCoFix HiSort HiProd HiInd HCheck ; unfold env_prop_bd.
+      pose (@Fix_F typing_sum (precompose lt typing_sum_size) Ptyping_sum) as p.
     forward p.
-    2:{ intros Σ wfΣ.
-      enough (HP : forall x : typing_sum Σ wfΣ, Ptyping_sum x).
-      - repeat split ; intros.
-        + exact (HP (env_cons Σ wfΣ)).
-        + exact (HP (context_cons Σ wfΣ Γ wfΓ)).
-        + exact (HP (check_cons Σ wfΣ Γ T t X)).
-        + exact (HP (inf_cons Σ wfΣ Γ T t X)).
-        + exact (HP (sort_cons Σ wfΣ Γ t u X)).
-        + exact (HP (prod_cons Σ wfΣ Γ t na A B X)).
-        + exact (HP (ind_cons Σ wfΣ Γ ind t u args X)).
-      - intros x ; apply (p (Σ ; (wfΣ ; x))).
-        apply wf_dlexprod ; intros ; apply wf_precompose ; apply lt_wf.
+    2:{
+    enough (HP : forall x : typing_sum, Ptyping_sum x).
+    - repeat split ; intros.
+      + exact (HP (context_cons Γ wfΓ)).
+      + exact (HP (check_cons Γ T t X)).
+      + exact (HP (inf_cons Γ T t X)).
+      + exact (HP (sort_cons Γ t u X)).
+      + exact (HP (prod_cons Γ t na A B X)).
+      + exact (HP (ind_cons Γ ind t u args X)).
+    - intros x ; apply p.
+      apply wf_precompose ; apply lt_wf.
     }
     clear p.     
-    intros (Σ & wfΣ & d) IH'. simpl.
-    match goal with | IH' : forall y : _ , ?P _ _ -> _ |- _ =>
-      have IH : forall (Σ' : global_env_ext) (wfΣ' : wf Σ'.1) (d' :typing_sum Σ' wfΣ'),
-        P (Σ'; wfΣ'; d') (Σ; wfΣ; d) -> Ptyping_sum d' end.
-    1: intros Σ' wfΣ' d' H; exact (IH' (Σ' ; wfΣ' ; d') H).
-    clear IH'.
+    intros d IH.
     destruct d ; simpl.
-    4: destruct i.
-    - destruct Σ as [Σ φ]. destruct Σ.
-      1: constructor.
-      destruct p.
-      cbn in  *.
-      have IH' : forall Σ' wfΣ' (d' : typing_sum Σ' wfΣ'), globenv_size (Σ'.1) < S (globenv_size Σ) ->
-                    Ptyping_sum d'
-        by intros ; apply IH ; constructor ; simpl ; assumption.
-      clear IH.
-      inversion_clear wfΣ as [|? ? ? wfΣ' ? ? ? wfg].
-      constructor.
-      + change (Forall_decls_sorting Pcheck Psort (Σ,φ).1).
-        applyIH.
-      + assumption.
-      + assumption.
-      + destruct g as [[? [] ?]| ]; cbn.
-        * inversion wfg as [[] ?].
-          split.
-          1: eexists.
-          all: applyIH.
-          eassumption.
-        * inversion wfg.
-          eexists. applyIH.
-          eassumption.
-        * inversion wfg.
-          constructor.
-          3-5: assumption.
-          2:{
-            clear - wfΣ' IH' onParams0.
-            induction onParams0.
-            1: by constructor.
-            -- constructor.
-               1: by assumption.
-               destruct t0.
-               eexists.
-               applyIH.
-               by eassumption. 
-            -- constructor.
-               1: by assumption.
-               destruct t0.
-               constructor.
-               2: by cbn ; applyIH.
-               destruct l.
-               eexists.
-               applyIH.
-               by eassumption. 
-          }
-
-          remember (ind_bodies m) as Γ in onInductives0 |- *.
-          clear - wfΣ' IH' onParams0 onInductives0.
-          induction onInductives0 as [| ? ? ? [] ?].
-          1: by constructor.
-          constructor.
-          2: eassumption.
-          econstructor ; try eassumption.
-          ++ destruct onArity0.
-            eexists. applyIH.
-            eassumption.
-          ++ clear - wfΣ' IH' onConstructors0 onParams0.
-            induction onConstructors0.
-            1: by constructor.
-            constructor.
-            2: assumption.
-            destruct r.
-            constructor.
-            all: try assumption.
-            ** cbn.
-                destruct on_ctype0.
-                eexists.
-                applyIH.
-                eassumption.
-            ** eapply type_local_ctx_impl.
-                1: eassumption.
-                all: intros ; applyIH ; eapply type_local_ctx_wf_local ; try eassumption.
-
-            ** clear - wfΣ' IH' onParams0 on_cargs0 on_cindices0.
-               induction on_cindices0.
-               all: constructor ; auto.
-               1: destruct l ; eexists.
-               2: cbn.
-               all: applyIH.
-               eassumption.
-
-          ++ clear - wfΣ' IH' ind_sorts0 onParams0.
-              red in ind_sorts0 |- *.
-              destruct (universe_family ind_sort0).
-              all: intuition.
-              all: destruct indices_matter ; auto.
-              ** eapply type_local_ctx_impl.
-                1: eassumption.
-                all: intros ; applyIH ; eapply type_local_ctx_wf_local ; eassumption.
-              ** eapply type_local_ctx_impl.
-                1: eassumption.
-                all: intros ; applyIH ; eapply type_local_ctx_wf_local ; eassumption.
-
-
+    3: destruct i.
+    
     - apply HΓ.
-      1: assumption.
-      1:{ applyIH. constructor 2. simpl. apply wf_local_size_pos. }
       dependent induction wfΓ.
       + constructor.
       + destruct t0 as (u & d).
         constructor.
         * apply IHwfΓ.
         intros ; apply IH.
-        dependent destruction H ; [constructor | constructor 2] ; auto.
-        etransitivity ; eauto.
-        simpl ; cbn in d ; pose proof (infering_sort_size_pos d) ; lia.
-        * simpl ; red ; applyIH.
-          constructor 2. simpl.
-          have ? : 0 < wfl_size wfΓ by apply wf_local_size_pos.
+        simpl in *. lia.
+        
+        * simpl. red.
+          applyIH.
+          simpl.
+          assert (0 < wfl_size wfΓ) by apply All_local_env_sorting_size_pos.
+          simpl.
           lia.
-      + destruct t0 as [[u h] h'].
+      + destruct t0 as [u h].
         constructor.
-        2: constructor.
         * apply IHwfΓ.
           intros ; apply IH.
-          dependent destruction H ; [constructor | constructor 2] ; auto.
-          etransitivity ; eauto.
-          simpl.
-          cbn in h. pose proof (infering_sort_size_pos h). lia.
-        * red ; applyIH. constructor 2. cbn in h' |- *. pose proof (checking_size_pos h'). lia.
-        * red ; applyIH. constructor 2. cbn in h |- *. pose proof (infering_sort_size_pos h). lia.
+          simpl in *. pose proof (infering_sort_size_pos h). lia.
+        * red. applyIH. pose proof (infering_sort_size_pos h). simpl in *. lia.
+        * red. applyIH. pose proof (checking_size_pos t1). simpl in *. lia.
 
     - destruct c.
       unshelve (eapply HCheck ; eauto) ; auto.
-      1: eapply infering_wf_local ; eassumption.
       all: applyIH.
-      pose proof (infering_wf_local_size i).
-      lia.
 
     - unshelve eapply HRel ; auto.
       all: applyIH.
@@ -808,24 +524,16 @@ Section TypingInduction.
       all: applyIH.
 
     - unshelve eapply HProd ; auto.
-      1: apply (infering_sort_wf_local i).
       all: applyIH.
-      pose proof (infering_sort_wf_local_size i). lia.
     
     - unshelve eapply HLambda ; auto.
-      1: apply (infering_sort_wf_local i).
       all: applyIH.
-      pose proof (infering_sort_wf_local_size i). lia.
 
     - unshelve eapply HLetIn ; auto.
-      1: apply (infering_sort_wf_local i).
       all: applyIH.
-      pose proof (infering_sort_wf_local_size i). lia.
 
-    - unshelve eapply (HApp _ _ _ _ _ _ _ A) ; auto.
-      2: apply (infering_prod_wf_local i).
+    - eapply HApp ; eauto.
       all: applyIH.
-      pose proof (infering_prod_wf_local_size i). lia.
 
     - unshelve eapply HConst ; auto.
       all: applyIH.
@@ -838,131 +546,96 @@ Section TypingInduction.
 
     - destruct indnpar as [ind' npar'] ; cbn in ind ; cbn in npar ; subst ind ; subst npar.
       unshelve eapply HCase ; auto.
-      1: apply (infering_indu_wf_local i).
-      1-5: applyIH.
-      1: pose proof (infering_indu_wf_local_size i) ; lia.
-      match goal with | IH : forall Σ' wfΣ' d', _ _ (_ ; _ ; ?d) -> _ |- _ =>
-        have IH' : forall d' : typing_sum Σ wfΣ, (typing_sum_size d') < (typing_sum_size d) -> Ptyping_sum d' end.
-      1:{ intros. apply IH. constructor 2. assumption. }
+      1-2: applyIH.
       remember btys as b in e2.
-      clear - IH'. cbn in IH' |- *.
+      clear Heqb.
+      cbn in IH.
       induction a.
       1: by constructor.
-      destruct r as [? [? ?]].
+      destruct r.
       constructor.
       + intuition eauto.
-        1: unshelve eapply (IH' (sort_cons _ wfΣ _ _ _ _)) ; try eassumption.
-        2: unshelve eapply (IH' (check_cons _ wfΣ _ _ _ _)) ; try eassumption.
-        all: simpl ; lia.
+        applyIH.
       + apply IHa.
-        intros. apply IH'. simpl in *. lia.
+        intros. apply IH. simpl in *. lia.
     
     - unshelve eapply HProj ; auto.
-      1: apply (infering_indu_wf_local i).
       all: applyIH.
-      pose proof (infering_indu_wf_local_size i). lia.
 
     - unshelve eapply HFix ; eauto.
-      1-2: applyIH.
 
-      all: have IH' : (forall d' : typing_sum Σ wfΣ,
-      (typing_sum_size d') <
-        (typing_sum_size (inf_cons _ wfΣ _ _ (tFix mfix n)
-        (infer_Fix Σ Γ mfix n decl i e a a0 a1 i0)))
-      -> Ptyping_sum d') by intros ; apply IH ; constructor 2 ; assumption.
-      all: simpl in IH'.
+      all: simpl in IH.
       all: remember (fix_context mfix) as mfixcontext.
 
-      1:{
-        remember (all_size _ _ a1) as s.
-        clear -IH'.
-        dependent induction a0.
+      + remember (all_size _ _ a0) as s.
+        clear -IH.
+        dependent induction a.
         1: by constructor.
         constructor ; cbn.
-        + destruct p ; eexists ; split.
+        * destruct p ; eexists ; split.
           1: eassumption.
-          unshelve eapply (IH' (sort_cons _ wfΣ _ _ _ _)).
-          all: try assumption.
-          simpl. lia.
-        + apply (IHa0 s).
+          applyIH.
+        * apply (IHa s).
           intros.
-          apply IH'.
+          apply IH.
           cbn. lia.
-      }
 
-      remember (all_size _ _ a0) as s.
-      clear -IH'.
-      induction a1 as [| ? ? [? ?]].
-      1: by constructor.
-      constructor.
-      + intuition.
-        unshelve eapply (IH' (check_cons _ wfΣ _ _ _ _)) ; try assumption.
-        simpl. lia.
-      + apply IHa1.
-        intros ; apply IH'.
-        cbn. lia.
+      + remember (all_size _ _ a) as s.
+        clear -IH.
+        induction a0.
+        1: by constructor.
+        constructor.
+        * intuition.
+          applyIH.
+        * apply IHa0.
+          intros.
+          apply IH.
+          cbn. lia.
 
     - unshelve eapply HCoFix ; eauto.
-      1-2: applyIH.
 
-      all: have IH' : (forall d' : typing_sum Σ wfΣ,
-      (typing_sum_size d') <
-        (typing_sum_size (inf_cons _ wfΣ _ _ (tCoFix mfix n)
-        (infer_CoFix Σ Γ mfix n decl i e a a0 a1 i0)))
-      -> Ptyping_sum d')
-      by intros ; apply IH ; constructor 2 ; assumption.
-      all: simpl in IH'.
+      all: simpl in IH.
       all: remember (fix_context mfix) as mfixcontext.
 
-      {
-        remember (all_size _ _ a1) as s.
-        clear -IH'.
-        dependent induction a0.
+      + remember (all_size _ _ a0) as s.
+        clear -IH.
+        dependent induction a.
         1: by constructor.
         constructor ; cbn.
-        + destruct p ; eexists ; split.
+        * destruct p ; eexists ; split.
           1: eassumption.
-          unshelve eapply (IH' (sort_cons _ wfΣ _ _ _ _)).
-          all: try assumption.
-          simpl. lia.
-        + apply (IHa0 s).
+          applyIH.
+        * apply (IHa s).
           intros.
-          apply IH'.
+          apply IH.
           cbn. lia.
-      }
 
-      remember (all_size _ _ a0) as s.
-      clear -IH'.
-      induction a1.
-      1: by constructor.
-      constructor.
-      + intuition.
-        unshelve eapply (IH' (check_cons _ wfΣ _ _ _ _)) ; try assumption.
-        simpl. lia.
-      + apply IHa1.
-        intros ; apply IH'.
-        cbn. lia.
+      + remember (all_size _ _ a) as s.
+        clear -IH.
+        induction a0 as [| ? ? ?].
+        1: by constructor.
+        constructor.
+        * intuition.
+          applyIH.
+        * apply IHa0.
+          intros.
+          apply IH.
+          cbn. lia.
 
     - destruct i.
       unshelve (eapply HiSort ; try eassumption) ; try eassumption.
-      1: eapply infering_wf_local ; eauto.
-      all: applyIH.
-      pose proof (infering_wf_local_size i). lia.
+      all:applyIH.
 
     - destruct i.
       unshelve (eapply HiProd ; try eassumption) ; try eassumption.
-      1: eapply infering_wf_local ; eauto.
       all: applyIH.
-      pose proof (infering_wf_local_size i). lia.
 
     - destruct i.
       unshelve (eapply HiInd ; try eassumption) ; try eassumption.
-      1: eapply infering_wf_local ; eauto.
       all: applyIH.
-      pose proof (infering_wf_local_size i). lia.
 Qed.
 
-End TypingInduction.
+End BidirectionalInduction.
 
 
 Ltac my_rename_hyp h th :=
